hol-light/standard/ml_kernel/ml_hol_kernelScript.sml
@@ -996,6 +996,8 @@ val def = new_basic_definition_def |> m_translate
 val def = (INST_TYPE_def |> SIMP_RULE std_ss [LET_DEF]) |> m_translate
 val def = (INST_def |> SIMP_RULE std_ss [LET_DEF]) |> m_translate
 val def = new_basic_type_definition_def |> m_translate
+val def = holKernelPmatchTheory.SYM_def |> m_translate
+val def = PROVE_HYP_def |> m_translate
 
 val kernel_thm = finalise_module_translation ();
 val _ = save_thm("kernel_thm", Q.SPEC `NONE` kernel_thm);
